# POS Example

- $F(x_1, x_2, x_3) = m_3 + m_4 + m_6 + m_7$
    - SOP
        
         $\sum m(3,4,6,7) = m_3 + m_4 + m_6 + m_7 \\
        = x_1'x_2x_3 + x_1x_2'x_3' + x_1x_2x_3' + x_1x_2x_3 \\
        = (x_1+x_1')x_2x_3 + (x_2+x_2')x_1x_3' \\
        = x_2x_3 + x_1x_3'$
        
    - POS
        
         $\Pi M(0,1,2,5)= M_0 + M_1 + M_2 + M_5 \\
        = (x_1+x_2+x_3)\cdot(x_1+x_2+x_3') \cdot(x_1+x_2'+x_3)\cdot ( x_1'+x_2+x_3') \\
        = (x_1+x_3)(x_2+x_3')$
        
- $F(x_1, x_2, x_3) =m_1 + m_3 + m_4 + m_6 + m_7$
    - SOP $= m_1 + m_3 + m_4 + m_6 + m_7 \\
    = x_1'x_2'x_3 + x_1'x_2x_3 + x_1x_2'x_3' + x_1x_2x_3' + x_1x_2x_3 \\
    = x_1'x_3(x_2+x_2')+x_1x_3'(x_2+x_2')+x_1x_2x_3\\
    =x_1'x_3+x_1x_3'+x_1x_2x_3$
    - POS $= M_0 + M_2 + M_5 \\
    = (x_1+x_2+x_3) \cdot(x_1+x_2'+x_3)\cdot ( x_1'+x_2+x_3') \\
    = (x_1+x_3)(x_2+x_3')$
- $F(x_1, x_2, x_3) =M_0 \cdot M_5$
    - SOP
        
        $m_2 + m_3 + m_6 + m_7 = 
        x_1{\prime}x_2x_3{\prime} + x_1{\prime}x_2x_3 + x_1x_2x_3{\prime} + x_1x_2x_3 \\
        = x_2x_3{\prime} + x_2x_3$
        
    - POS
        
        $M_0 \cdot M_5 = 
        (x_1 + x_2 + x_3) \cdot (x_1{\prime} + x_2 + x_3{\prime})\\ = (x_2 + x_3) \cdot (x_1 + x_3{\prime})$
        
- $F(x_1, x_2, x_3) =M_0 \cdot M_1 \cdot M_5 \cdot M_7$
    - SOP
        
        
        $F(x_1, x_2, x_3) = m_2 + m_3 + m_4 + m_6\\
        = x_1{\prime}x_2x_3{\prime} + x_1{\prime}x_2x_3 + x_1x_2{\prime}x_3{\prime} + x_1x_2x_3{\prime}\\
        =x_1{\prime}x_2(x_3{\prime} + x_3)+x_1x_3{\prime}(x_2{\prime} + x_2)\\
        =x_1{\prime}x_2 + x_1x_3{\prime}$
        
    - POS
        
        $F(x_1, x_2, x_3) = M_0 \cdot M_1 \cdot M_5 \cdot M_7 \\
        =(x_1 + x_2 + x_3) \cdot (x_1 + x_2 + x_3{\prime}) \cdot (x_1{\prime} + x_2 + x_3{\prime}) \cdot (x_1{\prime} + x_2{\prime} + x_3{\prime}) \\
        = (x_1 + x_2)\cdot(x_1{\prime} + x_3{\prime})$
        
